bugs/bug_5b.fst
@@ -1,0 +1,20 @@
+module Bug5
+
+type form =
+| FForall : (heap -> Tot form) -> form
+
+type deduce : form -> Type =
+  | DForallElim :
+             f:(heap->Tot form) ->
+             deduce (FForall f) ->
+             x:heap ->
+             deduce (f x)
+
+type pred = heap -> Tot form
+
+val hoist : pred -> heap -> Tot form
+let hoist p = fun h -> p h
+
+val hoare_consequence : p:pred -> deduce (FForall (hoist p)) -> h:heap -> Tot unit
+let hoare_consequence p vpp' h0 = 
+  ignore(DForallElim (hoist p) vpp' h0)
